---
title: "Home Work 1"
format: pdf
editor: visual
---

## Question (1) Math Review (25 points)

### Question (1_1): $f(x,y,z) = 3x^2 + sin(y)z$, I need to find partial derivatives for each x,y, and z:

Solution:

With respect to x: $\frac{\partial{f(x,y,z)}}{\partial{x}}$ = $6x$, everything else is constant ($sin(y)z$) as they are not function of x.

With respect to y: $\frac{\partial{f(x,y,z)}}{\partial{y}}$ = $z\cos(y)$, the first term ($3x^2$) derivative is zero in this case.

With respect to z: $\frac{\partial{f(x,y,z)}}{\partial{z}}$ = $\sin(y)$, the first term ($3x^2$) derivative is also zero in this case and ($sin(y)$) is treated as constant when deriving for z.

### Question (1_2): In this question, I will need to find the $\nabla f(x,y,z)$:

Using the results from the previous question,

$\nabla f(x,y,z)$= $\begin{bmatrix}
6x \\
z\cos(y) \\
\sin(y)
\end{bmatrix}$

### Question (1_3): Here we are replicating 1 and 2 but $f(x) = 3x_1^2 + \sin(x_2)x3$:

$\nabla f(x_1,x_2,x_3)$ = $\begin{bmatrix}
6x_1 \\
x_3\cos(x_2) \\
\sin(x_2)
\end{bmatrix}$

### Question (1_4_A):In this part, I will need to get the derivative for $\|x\|_2^2$:

$\|x\|_2^2$ = $\sum_{i = 1}^{n}x_i^2$ = $x_1^2 + x_2^2 + ... + x_n^2$

In this case: $\frac{\partial{\|x\|_2^2}}{\partial{x}}$ = $\frac{\partial({x_1^2 + x_2^2 + ... + x_n^2})}{\partial{x_1}}$ + $\frac{\partial({x_1^2 + x_2^2 + ... + x_n^2})}{\partial{x_2}}$ + ... + $\frac{\partial({x_1^2 + x_2^2 + ... + x_n^2})}{\partial{x_n}}$

$\frac{\partial{\|x\|_2^2}}{\partial{x}}$ = $\begin{bmatrix}
2x_1 \\
2x_2 \\
... \\
2x_n
\end{bmatrix}$. This represents the partial derivative for each x.

### Question (1_4_B):In this part, I will need to get the derivative for $\|x\|_2$:

$\|x\|_2$ = $\sqrt(\sum_{i = 1}^{n}x_i^2)$ = $\sqrt (x_1^2) + \sqrt(x_2^2) + ... + \sqrt(x_n^2)$

To get this derivative, $\frac{\partial{\|x\|_2}}{\partial{x}}$, I will be using the chain rule assuming that a new function h(z) = $\sqrt z$, where z(x) = $\sum_{i = 1}^{n}x_i^2$.

$\frac{\partial{h(z)}}{\partial{x}}$ = $\frac{\partial{h(z)}}{\partial{z}}$ \* $\frac{\partial{z(x)}}{\partial{x}}$

$\frac{\partial{h(z)}}{\partial{x}}$ = $\frac{1}{2\sqrt(\sum_{i = 1}^{n}x_i^2)}$ \* $\sum_{i=1}^{n}2x_i$

$\frac{\partial{h(z)}}{\partial{x}}$ = $\frac{x}{\|x\|_2}$

### Question (1_4_C):In this part, I will need to get the derivative for $\|x\|_1$:

$\|x\|_1$ = $\sum_{i = 1}^{n}|x_i|$ = $|x_1| + |x_2| + ... + |x_n|$

$\frac{\partial{\|x\|_1}}{\partial{x}}$: depends on the value of $x_i$. If $x_i$ positive, it would be 1, if negative, it would be -1, and undefined when $x_i$ equals zero. To represent the derivative of this function, the sign function can be used in this case:

$\mathrm{sgn}(x)$

$\frac{\partial{\|x\|_1}}{\partial{x}}$ = $\begin{bmatrix}
\mathrm{sgn}(x_1) \\
\mathrm{sgn}(x_2) \\
... \\
\mathrm{sgn}(x_n)
\end{bmatrix}$

### Question (1_4_D):In this part, I will need to get the derivative for $\|x\|\infty$:

$\|x\|\infty$ = $max|X_i|$, This entails many cases under the hood and can be represented using the sign function:

$\frac{\partial{\|x\|\infty}}{\partial{x_i}}$ = $\mathrm{sgn}(x_i)$ Accordingly, $\frac{\partial{\|x\|\infty}}{\partial{x_i}}$ = $[0,..., \mathrm{sgn}(x_i),...,0]^T$. Those components that are not achieving the maximum, the derivative is 0.

### Question (1_5): In this part, I will need to get the derivative of f(x) =$e^{\frac{-1}{2}\|x\|_2^2}$.

For this function, the chain rule will be used assuming a new function h(z) = $e^{z}$, where z = ${\frac{-1}{2}\|x\|_2^2}$. In this case, we would be looking for:

$\frac{\partial{h(z)}}{\partial{x}}$ = $\frac{\partial{h(z)}}{\partial{z}}$ \* $\frac{\partial{z(x)}}{x}$

$\frac{\partial{h(z)}}{\partial{x}}$ = $e^{z}$ \* $-x_i$

$\frac{\partial{h(z)}}{\partial{x}}$ = $-x_i$ \*$e^{\frac{-1}{2}\|x_i\|_2^2}$ = \[$-x_1e^{\frac{-1}{2}\|x_1\|_2^2}$, $-x_2e^{\frac{-1}{2}\|x_2\|_2^2}$,..., $-x_ne^{\frac{-1}{2}\|x_n\|_2^2}$ \]

$\begin{bmatrix}
-x_1e^{\frac{-1}{2}\|x_1\|_2^2} \\
-x_2e^{\frac{-1}{2}\|x_2\|_2^2} \\
... \\
-x_ne^{\frac{-1}{2}\|x_n\|_2^2}
\end{bmatrix}$

### Question (1_6): In this part, I will need to get the two components of f(A,x):

In this case A is a 2x3 matrix= $A_{2x3}$ = $\begin{bmatrix}
  A1,1 & A1,2 & A1,3 \\
  A2,1 & A2,2 & A2,3 \\
\end{bmatrix}$

And $x_{1x3}$ = $\begin{bmatrix}
  x1 & x2 & x3
\end{bmatrix}$

f(A,x) = $Ax^T$ = $\begin{bmatrix}
  A1,1 & A1,2 & A1,3 \\
  A2,1 & A2,2 & A2,3 \\
\end{bmatrix}$ \* $\begin{bmatrix}
  x1 \\
  x2 \\
  x3
\end{bmatrix}$

f(A,x) = $Ax^T$ = $\begin{bmatrix}
  A1,1*x1 + A1,2*x2 + A1,3*x3 \\
  A2,1*x1 + A2,2*x2 + A2,3*x3
\end{bmatrix}$

### Question (1_7): In this part,I would need to get $\frac{\partial{f(A,x)_1}}{\partial{x}}$ and $\frac{\partial{f(A,x)_2}}{\partial{x}}$.

$\frac{\partial{f(A,x)_1}}{\partial{x}}$ = $\begin{bmatrix}
  A1,1 \\
  A1,2 \\
  A1,3
\end{bmatrix}$

$\frac{\partial{f(A,x)_2}}{\partial{x}}$ = $\begin{bmatrix}
  A2,1 \\
  A2,2 \\
  A2,3
\end{bmatrix}$

### Question (1_8): In this part,I would need to get

$\frac{\partial{f(A,x)}}{\partial{x}}$: Using results from the previous question, The result will be:

$\frac{\partial{f(A,x)}}{\partial{x}}$ = $\begin{bmatrix}
  A1,1 & A2,1 \\
  A1,2 & A2,2 \\
  A1,3 & A2,3
\end{bmatrix}$

### Question (1_9): In this part,I would need to get the derivative of

$\mathbb{E}[f(x)]$.

Given that: $\mathbb{E}[f(x)]$ = $\sum\Pr(X = x) f(x)$, then:

$\frac{\partial{\mathbb{E}[f(x)]}}{\partial{x}}$ = $\frac{\partial}{\partial{x}}\sum \Pr(X=x) f(x)$, note that $\Pr(X=x)$ is constant with respect to x.

$\frac{\partial{\mathbb{E}[f(x)]}}{\partial{x}}$ = $\sum\Pr(X=x) \frac{\partial}{\partial{x}} f(x)$.

### Question (2): Linear Algebra Output

![Performance comparison](%22/Users/alghwiri/Library/CloudStorage/OneDrive-UniversityofPittsburgh/Drive%20Back-up/Acadmics/HDS%20masters/Taken%20Courses/Deep%20learning/linear_algebra.png%22)
